Prefix: : <https://openenergy-platform.org/ontology/oeo_geo/>
Prefix: bfo: <http://purl.obolibrary.org/obo/bfo/2.0/bfo.owl#>
Prefix: dc: <http://purl.org/dc/elements/1.1/>
Prefix: oeo: <http://openenergy-platform.org/ontology/v0.0.1/oeo/>
Prefix: owl: <http://www.w3.org/2002/07/owl#>
Prefix: rdf: <http://www.w3.org/1999/02/22-rdf-syntax-ns#>
Prefix: rdfs: <http://www.w3.org/2000/01/rdf-schema#>
Prefix: xml: <http://www.w3.org/XML/1998/namespace>
Prefix: xsd: <http://www.w3.org/2001/XMLSchema#>



Ontology: <https://openenergy-platform.org/ontology/oeo_geo/>
<https://openenergy-platform.org/ontology/v0.0.1/oeo_geo/>
Import: <http://purl.obolibrary.org/obo/bfo/2.0/bfo.owl>

Annotations: 
    dc:contributor "Christian Winger",
    dc:contributor "Fabian Neuhaus",
    dc:contributor "Hannah Förster",
    dc:contributor "Lukas Emele",
    dc:contributor "Martin Glauer",
    dc:contributor "Sebastian Cordes",
    <http://purl.org/dc/terms/title> "Open Energy Ontology",
    rdfs:comment "Include description of the ontology (in particular its scope) here ..."

AnnotationProperty: <http://purl.obolibrary.org/obo/IAO_0000112>

    
AnnotationProperty: <http://purl.obolibrary.org/obo/IAO_0000115>

    
AnnotationProperty: <http://purl.obolibrary.org/obo/IAO_0000119>

    
AnnotationProperty: <http://purl.org/dc/terms/title>

    
AnnotationProperty: dc:contributor

    
AnnotationProperty: definition

    SubPropertyOf: 
        rdfs:comment
    
    
AnnotationProperty: rdfs:comment

    
AnnotationProperty: rdfs:isDefinedBy

    
AnnotationProperty: rdfs:label

    
Datatype: rdf:PlainLiteral

    
ObjectProperty: owl:topObjectProperty

    
ObjectProperty: oeo:part_of

    
Class: <http://purl.obolibrary.org/obo/BFO_0000002>

    
Class: <http://purl.obolibrary.org/obo/BFO_0000003>

    
Class: <http://purl.obolibrary.org/obo/BFO_0000015>

    
Class: <http://purl.obolibrary.org/obo/BFO_0000031>

    
Class: AdministrativeDivision

    Annotations: 
        <http://purl.obolibrary.org/obo/IAO_0000115> "An administrative division, unit, entity, area or region, also referred to as a subnational entity, statoid, constituent unit, or country subdivision, is a portion of a country or other region delineated for the purpose of administration. Administrative divisions are granted a certain degree of autonomy and are usually required to manage themselves through their own local governments. Countries are divided up into these smaller units to make managing their land and the affairs of their people easier. A country may be divided into provinces, which, in turn, are divided into counties, which, in turn, may be divided in whole or in part into municipalities."@en,
        <http://purl.obolibrary.org/obo/IAO_0000119> "https://en.wikipedia.org/w/index.php?title=Administrative_division&oldid=867063518"@en
    
    SubClassOf: 
        GeographicRegion
    
    
Class: City

    Annotations: 
        <http://purl.obolibrary.org/obo/IAO_0000119> "Eurostat: 
https://ec.europa.eu/eurostat/statistics-explained/index.php?title=Glossary:City"@en,
        <http://purl.obolibrary.org/obo/IAO_0000115> "A city is a local administrative unit (LAU) where the majority of the population lives in an urban centre of at least 50 000 inhabitants. This is part of the EU-OECD functional urban area definition (EU-OECD FUA)."@en
    
    SubClassOf: 
        AdministrativeDivision,
        oeo:part_of some AdministrativeDivision
    
    
Class: Continent

    Annotations: 
        <http://purl.obolibrary.org/obo/IAO_0000119> "https://en.wikipedia.org/w/index.php?title=Continent&oldid=868603165"@en,
        <http://purl.obolibrary.org/obo/IAO_0000115> "A continent is one of several very large landmasses of the world. Generally identified by convention rather than any strict criteria, up to seven regions are commonly regarded as continents."@en
    
    SubClassOf: 
        GeographicRegion
    
    
Class: Country

    Annotations: 
        <http://purl.obolibrary.org/obo/IAO_0000119> "https://en.wikipedia.org/w/index.php?title=Country&oldid=866952883"@en,
        <http://purl.obolibrary.org/obo/IAO_0000115> "A country is a region that is identified as a distinct national entity in political geography. A country may be an independent sovereign state or part of a larger state,[1] as a non-sovereign or formerly sovereign political division, or a geographic region associated with sets of previously independent or differently associated people with distinct political characteristics."@en
    
    SubClassOf: 
        AdministrativeDivision,
        oeo:part_of some AdministrativeDivision
    
    
Class: County

    Annotations: 
        <http://purl.obolibrary.org/obo/IAO_0000115> "A county is a geographical region of a country used for administrative or other purposes, in certain modern nations. The term is derived from the Old French conté or cunté denoting a jurisdiction under the sovereignty of a count (earl) or a viscount."@en,
        <http://purl.obolibrary.org/obo/IAO_0000119> "https://en.wikipedia.org/w/index.php?title=County&oldid=868471406"@en
    
    SubClassOf: 
        AdministrativeDivision,
        oeo:part_of some AdministrativeDivision
    
    
Class: GeographicRegion

    Annotations: 
        <http://purl.obolibrary.org/obo/IAO_0000115> "A geographic region is a delimited part of the earth."@en
    
    SubClassOf: 
        <http://purl.obolibrary.org/obo/BFO_0000031>
    
    
Class: LAU

    Annotations: 
        <http://purl.obolibrary.org/obo/IAO_0000115> "To meet the demand for statistics at a local level, Eurostat maintains a system of Local Administrative Units (LAUs) compatible with NUTS. These LAUs are the building blocks of the NUTS, and comprise the municipalities and communes of the European Union.

The LAUs are:

administrative for reasons such as the availability of data and policy implementation capacity;

a subdivision of the NUTS 3 regions covering the whole economic territory of the Member States;

appropriate for the implementation of local level typologies included in TERCET, namely the coastal area and DEGURBA classification.",
        <http://purl.obolibrary.org/obo/IAO_0000119> "https://ec.europa.eu/eurostat/web/nuts/local-administrative-units"
    
    SubClassOf: 
        StatisticalRegion,
        oeo:part_of some NUTS3
    
    
Class: LoadArea

    Annotations: 
        <http://purl.obolibrary.org/obo/IAO_0000115> "A load area is an area that contains energy consumption.

Source: https://wiki.openmod-initiative.org/wiki/Load_area"@en
    
    SubClassOf: 
        GeographicRegion
    
    
Class: Municipality

    Annotations: 
        rdfs:label "Community"@en,
        rdfs:label "Municipality"@en,
        <http://purl.obolibrary.org/obo/IAO_0000119> "https://en.wikipedia.org/w/index.php?title=Municipality&oldid=868484965"@en,
        <http://purl.obolibrary.org/obo/IAO_0000115> "A municipality is usually a single urban administrative division having corporate status and powers of self-government or jurisdiction as granted by national and state laws to which it is subordinate. It is to be distinguished (usually) from the county, which may encompass rural territory or numerous small communities such as towns, villages and hamlets."@en
    
    SubClassOf: 
        AdministrativeDivision,
        oeo:part_of some AdministrativeDivision
    
    
Class: NUTS0

    SubClassOf: 
        StatisticalRegion
    
    
Class: NUTS1

    SubClassOf: 
        StatisticalRegion,
        oeo:part_of some NUTS0
    
    
Class: NUTS2

    SubClassOf: 
        StatisticalRegion,
        oeo:part_of some NUTS1
    
    
Class: NUTS3

    SubClassOf: 
        StatisticalRegion,
        oeo:part_of some NUTS2
    
    
Class: Province

    Annotations: 
        <http://purl.obolibrary.org/obo/IAO_0000115> "A province is almost always an administrative division within a country or state. The term derives from the ancient Roman provincia, which was the major territorial and administrative unit of the Roman Empire's territorial possessions outside Italy. The term province has since been adopted by many countries. In some countries with no actual provinces, \"the provinces\" is a metaphorical term meaning \"outside the capital city\"."@en,
        <http://purl.obolibrary.org/obo/IAO_0000119> "https://en.wikipedia.org/w/index.php?title=Province&oldid=865815503"@en
    
    SubClassOf: 
        AdministrativeDivision,
        oeo:part_of some AdministrativeDivision
    
    
Class: StatisticalRegion

    SubClassOf: 
        GeographicRegion
    
    
Individual: Africa

    Annotations: 
        <http://purl.obolibrary.org/obo/IAO_0000119> "https://en.wikipedia.org/w/index.php?title=Africa&oldid=876942469",
        <http://purl.obolibrary.org/obo/IAO_0000115> "Africa is the world's second largest and second most-populous continent (behind Asia in both categories). At about 30.3 million km2 (11.7 million square miles) including adjacent islands, it covers 6% of Earth's total surface area and 20% of its land area."
    
    Types: 
        Continent
    
    
Individual: Ampere

    Annotations: 
        rdfs:comment "Unit symbol: A
SI unit for electric current."@en
    
    
Individual: Antarctica

    Annotations: 
        <http://purl.obolibrary.org/obo/IAO_0000115> "Antarctica is Earth's southernmost continent. It contains the geographic South Pole and is situated in the Antarctic region of the Southern Hemisphere, almost entirely south of the Antarctic Circle, and is surrounded by the Southern Ocean. At 14,000,000 square kilometres (5,400,000 square miles), it is the fifth-largest continent.",
        <http://purl.obolibrary.org/obo/IAO_0000119> "https://en.wikipedia.org/w/index.php?title=Antarctica&oldid=877196656"
    
    Types: 
        Continent
    
    
Individual: Asia

    Annotations: 
        <http://purl.obolibrary.org/obo/IAO_0000119> "https://en.wikipedia.org/w/index.php?title=Asia&oldid=876007948",
        <http://purl.obolibrary.org/obo/IAO_0000115> "Asia is Earth's largest and most populous continent, located primarily in the Eastern and Northern Hemispheres. It shares the continental landmass of Eurasia with the continent of Europe and the continental landmass of Afro-Eurasia with both Europe and Africa. Asia covers an area of 44,579,000 square kilometres (17,212,000 sq mi), about 30% of Earth's total land area and 8.7% of the Earth's total surface area."
    
    Types: 
        Continent
    
    
Individual: Australia

    Annotations: 
        <http://purl.obolibrary.org/obo/IAO_0000115> "The continent of Australia, sometimes known in technical contexts by the names Sahul, Australinea or Meganesia to distinguish it from the country of Australia, consists of the land masses which sit on Australia's continental shelf. This includes mainland Australia, Tasmania, and the island of New Guinea (comprising Papua New Guinea and two Indonesian provinces).[1] Situated in the geographical region of Oceania, it is the smallest of the seven traditional continents in the English conception.",
        <http://purl.obolibrary.org/obo/IAO_0000119> "https://en.wikipedia.org/w/index.php?title=Australia_(continent)&oldid=874016426"
    
    Types: 
        Continent
    
    
Individual: Coal

    
Individual: Common_year

    Annotations: 
        rdfs:comment "Unit symbol: a, y
1 a = 365 d"@en
    
    
Individual: Coulomb

    Annotations: 
        rdfs:comment "Unit symbol: C
SI unit for electric charge."@en
    
    
Individual: Day

    Annotations: 
        rdfs:comment "Unit symbol: d
1 d = 24 h = 1440 min = 86,400 s"@en
    
    
Individual: Europe

    Annotations: 
        <http://purl.obolibrary.org/obo/IAO_0000115> "Europe is a continent located entirely in the Northern Hemisphere and mostly in the Eastern Hemisphere. It is bordered by the Arctic Ocean to the north, the Atlantic Ocean to the west and the Mediterranean Sea to the south. It comprises the westernmost part of Eurasia.",
        <http://purl.obolibrary.org/obo/IAO_0000119> "https://en.wikipedia.org/w/index.php?title=Europe&oldid=876129250"
    
    Types: 
        Continent
    
    
Individual: False

    
Individual: Farad

    Annotations: 
        rdfs:comment "Unit symbol: F
SI derived unit of electrical capacitance."@en
    
    
Individual: Foot

    Annotations: 
        rdfs:comment "Unit symbol: ft
1 ft = 0.3048 m"@en
    
    
Individual: Germany

    Types: 
        Country
    
    
Individual: Grain

    Annotations: 
        rdfs:comment "Unit symbol: grain, gr
1 gr = 64,79891 mg"@en
    
    
Individual: Gram

    Annotations: 
        rdfs:comment "Unit symbol: g
SI unit for mass: kg (1 kg = 1000 g)"@en
    
    
Individual: HardCoal

    
Individual: Heat

    
Individual: Hour

    Annotations: 
        rdfs:comment "Unit symbol: h
1h = 60 min = 3600 s"@en
    
    
Individual: Inch

    Annotations: 
        rdfs:comment "Unit symbol: in, \"
1 in = 1\" = 2,54 cm = 0,0254 m"@en
    
    
Individual: Joule

    Annotations: 
        rdfs:comment "SI unit for energy.
Unit symbol: J
1 J = 1 kg*(m/s)^2"@en
    
    
Individual: Julian_year

    Annotations: 
        rdfs:comment "Unit symbol: a, a_jul, y, y_jul
1 a = 365,25 d = 31,557,600 s"@en
    
    
Individual: Kilowatt_hour

    Annotations: 
        rdfs:comment "Unit symbol: kWh
1 kWh = 3600 kJ
Used for electricity"@en
    
    
Individual: Leap_year

    Annotations: 
        rdfs:comment "Unit symbol: a, y
1 a = 366 d"@en
    
    
Individual: Light

    
Individual: Lignite

    
Individual: Metre

    Annotations: 
        rdfs:comment "Unit symbol: m
SI unit for length"@en
    
    
Individual: Mile

    Annotations: 
        rdfs:comment "Unit symbol: mile
1 mile = 1609.344 m"@en
    
    
Individual: Minute

    Annotations: 
        rdfs:comment "Unit Symbol: min
1 min = 60s"@en
    
    
Individual: Nautical_mile

    Annotations: 
        rdfs:comment "Unit symbol: M, NM, nmi, sm
1 M = 1852 m"@en
    
    
Individual: Newton_metre

    Annotations: 
        rdfs:comment "Unit symbol: Nm
1 Nm = 1 J
Used for torque"@en
    
    
Individual: NorthAmerica

    Annotations: 
        <http://purl.obolibrary.org/obo/IAO_0000115> "North America is a continent entirely within the Northern Hemisphere and almost all within the Western Hemisphere; it is also considered by some to be a northern subcontinent of the Americas. It is bordered to the north by the Arctic Ocean, to the east by the Atlantic Ocean, to the west and south by the Pacific Ocean, and to the southeast by South America and the Caribbean Sea.",
        <http://purl.obolibrary.org/obo/IAO_0000119> "https://en.wikipedia.org/w/index.php?title=North_America&oldid=876018837"
    
    Types: 
        Continent
    
    
Individual: Nuclear

    
Individual: Ohm

    Annotations: 
        rdfs:comment "Unit symbol: Ω
SI derived unit for electrical resistance"@en
    
    
Individual: Oil

    
Individual: Ounce

    Annotations: 
        rdfs:comment "Unit symbol: oz
1 oz = 28.349523125 g (there are other ounces but this is the one that is used the most)"@en
    
    
Individual: Pound

    Annotations: 
        rdfs:comment "Unit symbol: lb
1 lb = 0.45359237 kg"@en
    
    
Individual: Second

    Annotations: 
        rdfs:comment "Unit symbol: s
SI unit of time"@en
    
    
Individual: SouthAmerica

    Annotations: 
        <http://purl.obolibrary.org/obo/IAO_0000119> "https://en.wikipedia.org/w/index.php?title=South_America&oldid=876836428",
        <http://purl.obolibrary.org/obo/IAO_0000115> "South America is a continent in the Western Hemisphere, mostly in the Southern Hemisphere, with a relatively small portion in the Northern Hemisphere."
    
    Types: 
        Continent
    
    
Individual: Therm

    Annotations: 
        rdfs:comment "Unit symbol: thm
1 thm ≈ 105.5 MJ (exact value depending on region)
Used for natural gas"@en
    
    
Individual: True

    
Individual: Volt

    Annotations: 
        rdfs:comment "Unit symbol: V
SI derived unit for voltage."@en
    
    
Individual: Water

    
Individual: Watt

    Annotations: 
        rdfs:comment "Unit symbol: W
SI derived unit for power."@en
    
    
Individual: Week

    Annotations: 
        rdfs:comment "Unit symbol: week
1 week = 7 d"@en
    
    
Individual: Wind

    
Individual: Yard

    Annotations: 
        rdfs:comment "Unit symbol: yd
1 yd = 0.9144 m"@en
    
    
